code/curve25519/Hacl.EC.Ladder.BigLoop.fst
@@ -42,7 +42,7 @@ val cmult_big_loop:
          let spointb0 : spoint_513 = (as_seq h0 (getx nqpq), (as_seq h0 (getz nqpq))) in
          (spointa1, spointb1) == cmult_big_loop_spec (as_seq h0 n) (spointa0) (spointb0) pointq i)
     ))
-#reset-options "--initial_fuel 1 --max_fuel 1 --z3rlimit 100"
+#reset-options "--initial_fuel 1 --max_fuel 1 --z3rlimit 1000"
 let rec cmult_big_loop n nq nqpq nq2 nqpq2 q i =
   if (U32.(i =^ 0ul)) then ()
   else (
@@ -50,6 +50,5 @@ let rec cmult_big_loop n nq nqpq nq2 nqpq2 q i =
     let i = U32.(i -^ 1ul) in
     let byte = n.(i) in
     cmult_small_loop nq nqpq nq2 nqpq2 q byte 8ul;
-    cmult_big_loop n nq nqpq nq2 nqpq2 q i;
-    admit()
+    cmult_big_loop n nq nqpq nq2 nqpq2 q i
   )
